checkpoint

sat.dfy
@@ -4,133 +4,296 @@ include "util.dfy"
 // inspired by https://siddhartha-gadgil.github.io/automating-mathematics/posts/sat-solving/
 newtype Variable = int
 
-datatype Expression = 
+datatype Exp =
     Constant(bool) |
     Var(Variable) |
     Not(Expression) |
     And(set<Expression>) |
     Or(set<Expression>) |
-    Implies(Expression, Expression) | 
+    Implies(Expression, Expression) |
     Equivalent(Expression, Expression)
-
-function children(e: Expression) : (cs: set<Expression>)
-    decreases e
-    ensures e !in cs
 {
-    match e {
-        case Constant(b) => {}
-        case Var(v) => {}
-        case Not(e) => {e}
-        case And(ands) => ands
-        case Or(ors) => ors
-        case Implies(a,b) => {a, b}
-        case Equivalent(a,b) => {a, b}
+    function children() : (cs: set<Expression>)
+    {
+        match this {
+            case Constant(b) => {}
+            case Var(v) => {}
+            case Not(e) => {e}
+            case And(ands) => ands
+            case Or(ors) => ors
+            case Implies(a,b) => {a, b}
+            case Equivalent(a,b) => {a, b}
+        }
+    }
+
+    predicate LocalValid()
+    {
+        match this {
+            case Constant(b) => true
+            case Var(v) => true
+            case Not(e) => true
+            case And(ands) => |ands| >= 1
+            case Or(ors) => |ors| >= 1
+            case Implies(a,b) => true
+            case Equivalent(a,b) => true
+        }
+    }
+
+    // function vars() : (vs: set<Variable>)
+    //     requires this.Valid()
+    //     decreases this.height
+    //     ensures forall i :: i in this.exp.children() ==> vs >= i.vars()
+    // {
+    //     match exp {
+    //         case Constant(b) => {}
+    //         case Var(v) => {v}
+    //         case Not(e) => e.vars()
+    //         case And(ands) => flatten(set a | a in ands :: a.vars())
+    //         case Or(ors) => flatten(set o | o in ors :: o.vars())
+    //         case Implies(a,b) => a.vars() + b.vars()
+    //         case Equivalent(a,b) => a.vars() + b.vars()
+    //     }
+    // }
+
+    function height() : int
+        requires LocalValid()
+    {
+        match this {
+            case Constant(b) => 0
+            case Var(v) => 0
+            case Not(e) => e.height + 1
+            case And(ands) =>
+                var heights := map_set(ands, (i: Expression) => i.exp.height());
+                max(heights) + 1
+            case Or(ors) => max(set i | i in ors :: i.height) + 1
+            case Implies(a,b) => max({a.height, b.height}) + 1
+            case Equivalent(a,b) => max({a.height, b.height}) + 1
+        }
     }
 }
 
-function descendents(e: Expression) : (d: set<Expression>)
-    decreases e
-    ensures e !in d
-    ensures children(e) <= d
-    ensures forall i :: i in d ==> height(e) > height(i)
-    ensures forall i :: i in children(e) ==> descendents(i) < d
+function make_exp(exp: Exp) : (e: Expression)
+    requires forall c :: c in exp.children() ==> c.Valid()
+    ensures e.Valid()
 {
-    match e {
-        case Constant(b) => {}
-        case Var(v) => {}
-        case Not(x) => {x} + descendents(x)
-        case And(s) => s + flatten(set i | i in s :: descendents(i))
-        case Or(s) => s + flatten(set i | i in s :: descendents(i))
-        case Implies(a,b) => {a, b} + descendents(a) + descendents(b)
-        case Equivalent(a,b) => {a, b} + descendents(a) + descendents(b)
+    var h := if |exp.children()| == 0 then
+        0
+    else
+        var heights_set := map_set(exp.children(), (c: Expression) => c.height);
+        var max_child := max(heights_set);
+        max_child + 1;
+    Expression(h, exp)
+}
+
+datatype Expression = Expression(height: int, exp: Exp)
+{
+    ghost predicate Valid()
+        decreases this.height
+    {
+        this.height >= 0 &&
+        if this.height == 0 then
+            |this.exp.children()| == 0
+        else
+            forall c :: c in this.exp.children() ==>
+                this.height > c.height &&
+                c.Valid()
+    }
+ 
+
+
+    function eval(vs: map<Variable,bool>) : bool
+        requires this.Valid()
+        requires vs.Keys >= this.vars()
+        decreases this.height
+    {
+        match exp {
+            case Constant(b) => b
+            case Var(v) => vs[v]
+            case Not(e) => !e.eval(vs)
+            case And(ands) => forall a :: a in ands ==> a.eval(vs)
+            case Or(ors) => !(forall o :: o in ors ==> !o.eval(vs))
+            case Implies(a,b) => !a.eval(vs) || b.eval(vs)
+            case Equivalent(a,b) => (a.eval(vs) && b.eval(vs)) || (!a.eval(vs) && !b.eval(vs))
+        }
+    }
+
+ 
+
+    // lemma descendent_vars(e: Expression, vs: set<Variable>)
+    //     requires e.vars() == vs
+    //     decreases e.height
+    //     //ensures forall i :: i in descendents(e) ==> vars(e) >= vars(i)
+    // {
+    //     assert forall i :: i in e.exp.children() ==> e.vars() >= i.vars();
+    //     var cs := e.exp.children();
+    //     var cds := flatten(set i | i in e.exp.children() :: i.descendents());
+    //     var ds := e.descendents();
+    //     //assert cds < ds;
+
+    //     var cds_vs := set_vars(cds);
+    //     var ds_vs := set_vars(ds);
+    // }
+
+    function descendents() : (d: set<Expression>)
+        requires this.Valid()
+        decreases this.exp
+        ensures this.exp.children() <= d
+        ensures forall i :: i in d ==> this.height > i.height
+        ensures forall i :: i in this.exp.children() ==> descendents() < d
+    {
+        match exp {
+            case Constant(b) => {}
+            case Var(v) => {}
+            case Not(x) => {x} + x.descendents()
+            case And(s) => s + flatten(set i | i in s :: i.descendents())
+            case Or(s) => s + flatten(set i | i in s :: i.descendents())
+            case Implies(a,b) => {a, b} + a.descendents() + b.descendents()
+            case Equivalent(a,b) => {a, b} + a.descendents() + b.descendents()
+        }
+    }
+
+    function simplify_one(vs: map<Variable,bool>) : (out: Expression)
+        requires vs.Keys >= this.vars()
+        decreases this
+        ensures match out.exp {
+            case Implies(_,_) => false
+            case Equivalent(_,_) => false
+            case Not(ee) =>
+                match ee.exp {
+                    case Or(_) => false
+                    case And(_) => false
+                    case _ => true
+                }
+            case e => true
+        }
+        ensures this.vars() >= out.vars()
+        ensures this.eval(vs) == out.eval(vs)
+    {
+        match this.exp {
+            case Implies(a,b) => make_exp(Or({make_exp(Not(a)), b}))
+            case Equivalent(a,b) =>
+                var both_true := make_exp(And({a,b}));
+                assert both_true.eval(vs) == (a.eval(vs) && b.eval(vs));
+                var first_false := make_exp(Not(a));
+                var second_false := make_exp(Not(b));
+                var both_false := make_exp(And({first_false, second_false}));
+                assert both_false.vars() <= this.vars();
+                assert both_false.eval(vs) == (!a.eval(vs) && !b.eval(vs));
+                var out := make_exp(Or({both_true, both_false}));
+                assert out.vars() <= this.vars();
+                assert this.eval(vs) == out.eval(vs);
+                out
+            case Not(n) =>
+                var out := make_exp(match n.exp {
+                    case Or(s) =>
+                        // n.exp.descendents_vars(vs);
+                        s.demorgan1(vs);
+                        make_exp(And(set i | i in s :: Not(i)))
+                    case And(s) =>
+                        // n.exp.descendents_vars(vs);
+                        s.demorgan2(vs);
+                        make_exp(Or(set i | i in s :: Not(i)))
+                    case _ => this
+                });
+                assert this.eval(vs) == out.eval(vs);
+                out
+            case e => e
+        }
+    }
+
+    lemma demorgan1(s: set<Exp>, vs: map<Variable,bool>)
+        requires forall i :: i in s ==> vs.Keys >= i.vars()
+        ensures 
+            make_exp(Not(make_exp(Or(s)))).eval(vs) == 
+            make_exp(And(set i | i in s :: make_exp(Not(i)))).eval(vs)
+    {
+        var x := make_exp(Not(make_exp(Or(s)))).eval(vs);
+        var or := make_exp(Or(s));
+        assert or.eval(vs) == (!forall i :: i in s ==> !i.eval(vs));
+        assert x == !(!forall i :: i in s ==> !i.eval(vs));
+
+        var y := make_exp(And(set i | i in s :: make_exp(Not(i)))).eval(vs);
+        var nots := set i | i in s :: make_exp(Not(i));
+        assert y == make_exp(And(nots)).eval(vs);
+        assert make_exp(And(nots)).eval(vs) == (forall i :: i in nots ==> i.eval(vs));
+        assert !(!forall i :: i in s ==> !i.eval(vs)) == (forall i :: i in s ==> make_exp(Not(i)).eval(vs));
     }
 }
 
-function child_descendents(e: Expression) : (cd_flat: set<Expression>)
-    ensures flatten(set i | i in children(e) :: descendents(i)) <= descendents(e)
-    ensures cd_flat == flatten(set i | i in children(e) :: descendents(i))
-{
-    child_descendents_helper(e, descendents(e))
-}
 
-function child_descendents_helper(e: Expression, d: set<Expression>) : (cd_flat: set<Expression>)
-    requires d == descendents(e)
-    ensures flatten(set i | i in children(e) :: descendents(i)) <= d
-    ensures cd_flat == flatten(set i | i in children(e) :: descendents(i))
-{
-    assert forall i :: i in children(e) ==> descendents(i) < d;
-    assert e !in d;
 
-    var cs := children(e);
-    assert forall i :: i in cs ==> descendents(i) < d;
-    assert cs == children(e);
-    var cd_flat := flatten(set i | i in cs :: descendents(i));
-    assert cd_flat == flatten(set i | i in children(e) :: descendents(i));
-    assert cd_flat + cs == d;
-    assert cd_flat <= d;
-    cd_flat
-}
+// function child_descendents(e: Expression) : (cd_flat: set<Expression>)
+//     ensures flatten(set i | i in children(e) :: descendents(i)) <= descendents(e)
+//     ensures cd_flat == flatten(set i | i in children(e) :: descendents(i))
+// {
+//     child_descendents_helper(e, descendents(e))
+// }
 
-function height(e: Expression) : (h: int)
-    decreases e
-    ensures h >= 0
-    ensures forall i :: i in children(e) ==> h > height(i)
-{       
-    match e {
-        case Constant(b) => 0
-        case Var(v) => 0
-        case Not(e) => height(e) + 1
-        case And(s) =>
-            if |s| == 0 then
-                0
-            else
-                assert s == children(e);
-                var heights_set := set i | i in s :: height(i);
-                var heights_map := map i | i in s :: height(i);
-                assert forall i :: i in s ==> height(i) in heights_set;
-                assert forall i :: i in s ==> i in heights_map.Keys;
-                assert forall i :: i in s ==> height(i) in heights_map.Values;
-                assert heights_set == heights_map.Values;
-                notempty(s, heights_map);
-                var max_child := max(heights_set);
-                var h := max_child + 1;
-                assert forall i :: i in children(e) ==> h > height(i);
-                h
-        case Or(s) => 
-            if |s| == 0 then
-                0
-            else
-                assert s == children(e);
-                var heights_set := set i | i in s :: height(i);
-                var heights_map := map i | i in s :: height(i);
-                assert forall i :: i in s ==> height(i) in heights_set;
-                assert forall i :: i in s ==> i in heights_map.Keys;
-                assert forall i :: i in s ==> height(i) in heights_map.Values;
-                assert heights_set == heights_map.Values;
-                notempty(s, heights_map);
-                var max_child := max(heights_set);
-                var h := max_child + 1;
-                assert forall i :: i in children(e) ==> h > height(i);
-                h
-        case Implies(a,b) => max({height(a), height(b)}) + 1
-        case Equivalent(a,b) => max({height(a), height(b)}) + 1
-    }
-}
+// function child_descendents_helper(e: Expression, d: set<Expression>) : (cd_flat: set<Expression>)
+//     requires d == descendents(e)
+//     ensures flatten(set i | i in children(e) :: descendents(i)) <= d
+//     ensures cd_flat == flatten(set i | i in children(e) :: descendents(i))
+// {
+//     assert forall i :: i in children(e) ==> descendents(i) < d;
+//     assert e !in d;
 
-function vars(e: Expression) : (vs: set<Variable>)
-    decreases e, height(e)
-    ensures forall i :: i in children(e) ==> vs >= vars(i)
-{
-    match e {
-        case Constant(b) => {}
-        case Var(v) => {v}
-        case Not(e) => vars(e)
-        case And(ands) => flatten(set a | a in ands :: vars(a))
-        case Or(ors) => flatten(set o | o in ors :: vars(o))
-        case Implies(a,b) => vars(a) + vars(b)
-        case Equivalent(a,b) => vars(a) + vars(b)
-    }
-}
+//     var cs := children(e);
+//     assert forall i :: i in cs ==> descendents(i) < d;
+//     assert cs == children(e);
+//     var cd_flat := flatten(set i | i in cs :: descendents(i));
+//     assert cd_flat == flatten(set i | i in children(e) :: descendents(i));
+//     assert cd_flat + cs == d;
+//     assert cd_flat <= d;
+//     cd_flat
+// }
+
+// function height(e: Expression) : (h: int)
+//     decreases e
+//     ensures h >= 0
+//     ensures forall i :: i in children(e) ==> h > height(i)
+// {
+//     match e {
+//         case Constant(b) => 0
+//         case Var(v) => 0
+//         case Not(e) => height(e) + 1
+//         case And(s) =>
+//             if |s| == 0 then
+//                 0
+//             else
+//                 assert s == children(e);
+//                 var heights_set := set i | i in s :: height(i);
+//                 var heights_map := map i | i in s :: height(i);
+//                 assert forall i :: i in s ==> height(i) in heights_set;
+//                 assert forall i :: i in s ==> i in heights_map.Keys;
+//                 assert forall i :: i in s ==> height(i) in heights_map.Values;
+//                 assert heights_set == heights_map.Values;
+//                 notempty(s, heights_map);
+//                 var max_child := max(heights_set);
+//                 var h := max_child + 1;
+//                 assert forall i :: i in children(e) ==> h > height(i);
+//                 h
+//         case Or(s) =>
+//             if |s| == 0 then
+//                 0
+//             else
+//                 assert s == children(e);
+//                 var heights_set := set i | i in s :: height(i);
+//                 var heights_map := map i | i in s :: height(i);
+//                 assert forall i :: i in s ==> height(i) in heights_set;
+//                 assert forall i :: i in s ==> i in heights_map.Keys;
+//                 assert forall i :: i in s ==> height(i) in heights_map.Values;
+//                 assert heights_set == heights_map.Values;
+//                 notempty(s, heights_map);
+//                 var max_child := max(heights_set);
+//                 var h := max_child + 1;
+//                 assert forall i :: i in children(e) ==> h > height(i);
+//                 h
+//         case Implies(a,b) => max({height(a), height(b)}) + 1
+//         case Equivalent(a,b) => max({height(a), height(b)}) + 1
+//     }
+// }
+
+
 /*
 function set_vars(s: set<Expression>) : (vs: set<Variable>)
     ensures forall i :: i in s ==> vars(i) <= vs
@@ -148,54 +311,13 @@ lemma bigger_set_bigger_vars(a: set<Expression>, b: set<Expression>, av: set<Var
 }
 /*
 
-lemma descendent_vars(e: Expression, vs: set<Variable>)
-    requires vars(e) == vs
-    decreases height(e)
-    //ensures forall i :: i in descendents(e) ==> vars(e) >= vars(i)
-{
-    assert forall i :: i in children(e) ==> vars(e) >= vars(i);
-    var cs := children(e);
-    var cds := flatten(set i | i in children(e) :: descendents(i));
-    var ds := descendents(e);
-    //assert cds < ds;
 
-    var cds_vs := set_vars(cds);
-    var ds_vs := set_vars(ds);
-
-}
 
 */
 
-function eval(e: Expression, vs: map<Variable,bool>) : bool
-    requires vs.Keys >= vars(e)
-    decreases e
-{
-    match e {
-        case Constant(b) => b
-        case Var(v) => vs[v]
-        case Not(e) => !eval(e, vs)
-        case And(ands) => forall a :: a in ands ==> eval(a, vs)
-        case Or(ors) => !(forall o :: o in ors ==> !eval(o, vs))
-        case Implies(a,b) => !eval(a, vs) || eval(b, vs)
-        case Equivalent(a,b) => (eval(a, vs) && eval(b,vs)) || (!eval(a, vs) && !eval(b, vs))
-    }
-}
 
-lemma demorgan1(s: set<Expression>, vs: map<Variable,bool>)
-    requires forall i :: i in s ==> vs.Keys >= vars(i)
-    ensures eval(Not(Or(s)), vs) == eval(And(set i | i in s :: Not(i)), vs)
-{
-    var x := eval(Not(Or(s)), vs);
-    var or := Or(s);
-    assert eval(or, vs) == (!forall i :: i in s ==> !eval(i, vs));
-    assert x == !(!forall i :: i in s ==> !eval(i, vs));
-    
-    var y := eval(And(set i | i in s :: Not(i)), vs);
-    var nots := set i | i in s :: Not(i);
-    assert y == eval(And(nots), vs);
-    assert eval(And(nots), vs) == (forall i :: i in nots ==> eval(i, vs));
-    assert !(!forall i :: i in s ==> !eval(i, vs)) == (forall i :: i in s ==> eval(Not(i), vs));
-}
+
+
 
 lemma demorgan2(s: set<Expression>, vs: map<Variable,bool>)
     requires forall i :: i in s ==> vs.Keys >= vars(i)
@@ -205,7 +327,7 @@ lemma demorgan2(s: set<Expression>, vs: map<Variable,bool>)
     var and := And(s);
     assert eval(and, vs) == (!forall i :: i in s ==> !eval(i, vs));
     assert x == !(!forall i :: i in s ==> !eval(i, vs));
-    
+
     var y := eval(Or(set i | i in s :: Not(i)), vs);
     var nots := set i | i in s :: Not(i);
     assert y == eval(Or(nots), vs);
@@ -213,56 +335,11 @@ lemma demorgan2(s: set<Expression>, vs: map<Variable,bool>)
     assert !(!forall i :: i in s ==> !eval(i, vs)) == (forall i :: i in s ==> eval(Not(i), vs));
 }
 
-function method simplify_one(e: Expression, vs: map<Variable,bool>) : (out: Expression)
-    requires vs.Keys >= vars(e)
-    decreases e
-    ensures match out {
-        case Implies(_,_) => false 
-        case Equivalent(_,_) => false
-        case Not(ee) =>
-            match ee {
-                case Or(_) => false
-                case And(_) => false
-                case _ => true
-            }
-        case e => true
-    }
-    ensures vars(e) >= vars(out)
-    ensures eval(e, vs) == eval(out, vs)
-{
-    match e {
-        case Implies(a,b) => Or({Not(a), b})
-        case Equivalent(a,b) => 
-            var both_true := And({a,b});
-            assert eval(both_true, vs) == (eval(a, vs) && eval(b, vs));
-            var both_false := And({Not(a),Not(b)});
-            assert vars(both_false) <= vars(e);
-            assert eval(both_false, vs) == (!eval(a, vs) && !eval(b, vs));
-            var out := Or({both_true, both_false});
-            assert vars(out) <= vars(e);
-            assert eval(e, vs) == eval(out, vs);
-            out
-        case Not(n) =>
-            var out := match n {
-                case Or(s) =>
-                    descendents_vars(e, vs);
-                    demorgan1(s, vs);
-                    And(set i | i in s :: Not(i))
-                case And(s) =>
-                    descendents_vars(e, vs);
-                    demorgan2(s, vs);
-                    Or(set i | i in s :: Not(i))
-                case _ => e
-            };
-            assert eval(e, vs) == eval(out, vs);
-            out
-        case e => e
-    }
-}
+
 
 predicate no_implies(e: Expression) {
     forall i :: i in {e} + descendents(e) ==> match i {
-        case Implies(_,_) => false 
+        case Implies(_,_) => false
         case e => true
     }
 }
@@ -282,12 +359,12 @@ function method simplify_implies(e: Expression, vs: map<Variable,bool>) : (out: 
         case Var(v) =>
             assert no_implies(e);
             e
-        case Not(x) => 
+        case Not(x) =>
             var xx := simplify_implies(x, vs);
             assert no_implies(xx);
             assert no_implies(Not(xx));
             Not(xx)
-        case And(s) => 
+        case And(s) =>
             var ss := set i | i in s :: simplify_implies(i, vs);
             assert forall i :: i in ss ==> no_implies(i);
             assert no_implies(And(ss));
@@ -297,14 +374,14 @@ function method simplify_implies(e: Expression, vs: map<Variable,bool>) : (out: 
             assert forall i :: i in ss ==> no_implies(i);
             assert no_implies(Or(ss));
             Or(ss)
-        case Implies(a,b) => 
+        case Implies(a,b) =>
             var a:= simplify_implies(a, vs);
             assert no_implies(a) && no_implies(Not(a));
             var b := simplify_implies(b, vs);
             assert no_implies(b);
             assert no_implies(Or({Not(a), b}));
             Or({Not(a), b})
-        case Equivalent(a,b) => 
+        case Equivalent(a,b) =>
             var a:= simplify_implies(a, vs);
             assert no_implies(a);
             var b := simplify_implies(b, vs);
@@ -318,7 +395,7 @@ function method simplify_implies(e: Expression, vs: map<Variable,bool>) : (out: 
 
 predicate no_equivalent(e: Expression) {
     forall i :: i in {e} + descendents(e) ==> match i {
-        case Equivalent(_,_) => false 
+        case Equivalent(_,_) => false
         case e => true
     }
 }
@@ -339,12 +416,12 @@ function method simplify_equivalent(e: Expression, vs: map<Variable,bool>) : (ou
         case Var(v) =>
             assert no_equivalent(e);
             e
-        case Not(x) => 
+        case Not(x) =>
             var xx := simplify_equivalent(x, vs);
             assert no_equivalent(xx);
             assert no_equivalent(Not(xx));
             Not(xx)
-        case And(s) => 
+        case And(s) =>
             var ss := set i | i in s :: simplify_equivalent(i, vs);
             assert forall i :: i in ss ==> no_equivalent(i);
             assert no_equivalent(And(ss));
@@ -354,10 +431,10 @@ function method simplify_equivalent(e: Expression, vs: map<Variable,bool>) : (ou
             assert forall i :: i in ss ==> no_equivalent(i);
             assert no_equivalent(Or(ss));
             Or(ss)
-        case Implies(a,b) => 
+        case Implies(a,b) =>
             assert false;
             a
-        case Equivalent(a,b) => 
+        case Equivalent(a,b) =>
             var a:= simplify_equivalent(a, vs);
             assert no_equivalent(a);
             var b := simplify_equivalent(b, vs);
@@ -397,7 +474,7 @@ function method simplify_not_expressions(e: Expression, vs: map<Variable,bool>) 
         case Var(v) =>
             assert no_not_expressions(e);
             e
-        case Not(x) => 
+        case Not(x) =>
             var xx := match x {
                 case Constant(b) =>
                     Constant(!b)
@@ -422,16 +499,16 @@ function method simplify_not_expressions(e: Expression, vs: map<Variable,bool>) 
                     var xx := And(set i | i in ss :: Not(i));
                     assert no_not_expressions(xx);
                     xx
-                case Implies(a,b) => 
+                case Implies(a,b) =>
                     assert false;
                     a
-                case Equivalent(a,b) => 
+                case Equivalent(a,b) =>
                     assert false;
                     a
             };
             assert no_not_expressions(xx);
             xx
-        case And(s) => 
+        case And(s) =>
             var ss := set i | i in s :: simplify_not_expressions(i, vs);
             assert forall i :: i in ss ==> no_not_expressions(i);
             assert no_not_expressions(And(ss));
@@ -441,10 +518,10 @@ function method simplify_not_expressions(e: Expression, vs: map<Variable,bool>) 
             assert forall i :: i in ss ==> no_not_expressions(i);
             assert no_not_expressions(Or(ss));
             Or(ss)
-        case Implies(a,b) => 
+        case Implies(a,b) =>
             assert false;
             a
-        case Equivalent(a,b) => 
+        case Equivalent(a,b) =>
             assert false;
             a
     };
