util.dfy
@@ -12,45 +12,52 @@ function flatten<T(!new)>(nested: set<set<T>>) : (f: set<T>)
     set x, y | y in nested && x in y :: x
 }
 
-function pick(s: set<int>): (x: int)
-  requires s != {}
-  ensures |s| == 1 ==> {x} == s
+lemma max_exists(s: set<int>)
+    requires |s| >= 1
+    ensures exists x :: x in s && forall y :: y in s ==> x >= y
 {
-    var x :| x in s; 
-    assert x in s;
-    if |s| == 1 then 
-        var remainder := s - {x};
-        assert |remainder| == 0;
-        assert remainder == {};
-        assert remainder + {x} == s;
-        assert {x} == s;
-        x
-    else
-        x
+    var max :| max in s;
+    var visited := {max};
+    var to_visit := s - visited;
+
+    while |to_visit| > 0
+        decreases |to_visit|
+        invariant forall x :: x in visited ==> max >= x
+        invariant visited + to_visit == s
+        invariant max in s
+    {
+        var x :| x in to_visit;
+        if x >= max {
+            max := x;
+        }
+
+        to_visit := to_visit - {x};
+        visited := visited + {x};
+    }
+
+    assert forall x :: x in visited ==> max >= x;
+    assert visited == s;
+    assert forall x :: x in s ==> max >= x;
+}
+
+lemma NotEmptySetHasNotEmptyMapping<A,B>(s: set<A>, f: (A) -> B, m: set<B>)
+    requires |s| >= 1
+    requires m == set i | i in s :: f(i)
+    ensures |m| >= 1
+{
+    var i :| i in s;
+    var y := f(i);
+    assert y in m;
 }
 
 function max(s: set<int>) : (m: int)
     requires |s| >= 1
-    decreases s
     ensures m in s
     ensures forall i :: i in s ==> m >= i
 {
-    var x := pick(s);
-    if |s| == 1 then
-        assert forall i :: i in s ==> x >= i;
-        x
-    else 
-        var remainder := s - {x};
-        var y:int := max(remainder);
-        if (x >= y) then 
-            assert forall i :: i in remainder ==> y >= i;
-            assert forall i :: i in remainder ==> x >= i;
-            assert s == {x} + remainder;
-            assert forall i :: i in s ==> x >= i;
-            x
-        else 
-            assert forall i :: i in s ==> y >= i;
-            y
+    max_exists(s);
+    var x :| x in s && forall y :: y in s ==> x >= y;
+    x
 }
 
 lemma notempty<K,V>(s: set<K>, m: map<K,V>)
@@ -58,3 +65,15 @@ lemma notempty<K,V>(s: set<K>, m: map<K,V>)
     ensures |s| == |m|
     ensures |s| >= 1 ==> |m| >= 1
 {}
+
+function map_set<A(!new),B>(x: set<A>, f: (A) -> B) :  (y: set<B>)
+    ensures |x| >= 1 ==> |y| >= 1
+    ensures y == (set i | i in x :: f(i))
+    ensures forall i :: i in x ==> f(i) in y
+{
+    var y := set i | i in x :: f(i);
+    ghost var ys_map := map i | i in x :: f(i);
+    assert x == ys_map.Keys;
+    assert y == ys_map.Values;
+    y
+}
